proof/security/PKE_ROM.ec
@@ -118,7 +118,7 @@ section.
 end section.
 
 module type OW_CPA_ADV = {
-  proc find(pk : pkey, c:ciphertext) : plaintext 
+  proc find(pk : pkey, c:ciphertext) : plaintext option
 }.
 
 clone FinType as MFinT with
@@ -141,7 +141,8 @@ module OW_CPA (S:Scheme, A: OW_CPA_ADV) = {
 
   proc main_perfect() = {
     var pk : pkey;
-    var m, m' : plaintext;
+    var m  : plaintext;
+    var m' : plaintext option;
     var cc : ciphertext;
     var sk : skey;
 
@@ -149,7 +150,7 @@ module OW_CPA (S:Scheme, A: OW_CPA_ADV) = {
     m        <$ dplaintext;
     cc       <@ S.enc(pk, m);
     m'       <@ A.find(pk,cc);
-    return (m' = m);
+    return (m' = Some m);
 
   }
 
@@ -163,8 +164,9 @@ module OW_CPA (S:Scheme, A: OW_CPA_ADV) = {
 
   proc main() : bool = {
     var pk : pkey;
-    var m, m' : plaintext;
-    var b;
+    var m  : plaintext;
+    var m' : plaintext option;
+    var b  : bool;
     var cc : ciphertext;
     var sk : skey;
 
@@ -172,14 +174,14 @@ module OW_CPA (S:Scheme, A: OW_CPA_ADV) = {
     m        <$ dplaintext;
     cc       <@ S.enc(pk, m);
     m'       <@ A.find(pk,cc);
-    b        <@ O.pco(sk, m',cc);
-    return b;
+    b        <@ O.pco(sk, oget m',cc);
+    return if m' = None then false else b;
   }
 }.
 
 module BOWp(S : Scheme, A :  OW_CPA_ADV) : CORR_ADV = {
    var m  : plaintext
-   var m' : plaintext
+   var m' : plaintext option
    var m'' : plaintext option
    var cc  : ciphertext
 
@@ -216,7 +218,7 @@ proof.
 move => A_ll Senc_ll Sdec_ll.
 have -> : 
   Pr[OW_CPA(S, A).main_perfect() @ &m : res] = 
-    Pr[ BOWp(S,A).main() @ &m : BOWp.m = BOWp.m' ].
+    Pr[ BOWp(S,A).main() @ &m : Some BOWp.m = BOWp.m' ].
 + byequiv => //.
   proc;inline *; seq 4 6 : #post; last by  conseq />;islossless.
   conseq  (_: _ ==> m{1} = BOWp.m{2} /\ m'{1} = BOWp.m'{2}); 1: by smt().
@@ -224,11 +226,11 @@ have -> :
 
 have -> : 
   Pr[OW_CPA(S, A).main() @ &m : res] = 
-    Pr[ BOWp(S,A).main() @ &m : Some BOWp.m' = BOWp.m'' ].
+    Pr[ BOWp(S,A).main() @ &m : if BOWp.m' = None then false else BOWp.m'' = BOWp.m'].
 + byequiv => //.
-  proc;inline *. seq 9 7 : #post; last by conseq />; islossless. 
-  wp; conseq (: m'0{1} = BOWp.m''{2} /\ m0{1} = BOWp.m'{2}); 1: smt().
-  by sim.
+  proc;inline *; seq 9 7 : #post; last by conseq />; islossless. 
+  wp. conseq (: m'{1} = BOWp.m'{2} /\ m'0{1} = BOWp.m''{2} /\ m0{1} = oget BOWp.m'{2}); 1: smt().
+  by call(:true);wp;call(:true);wp;call(:true);rnd;wp;call(:true);auto.
 
 have -> : 
   Pr[Correctness_Adv(S, BOWp(S, A)).main() @ &m : res] = 
@@ -248,8 +250,10 @@ end section.
 (* Ind implies ow for large message spaces *)
 
 module Bow(A :  OW_CPA_ADV) : Adversary = {
-   var m0, m1, m : plaintext
-   var pk : pkey
+   var m0, m1  : plaintext
+   var m       : plaintext option
+   var pk      : pkey
+
    proc choose(_pk : pkey) : plaintext * plaintext = {
      pk <- _pk;
      m0 <$ dplaintext;
@@ -261,9 +265,9 @@ module Bow(A :  OW_CPA_ADV) : Adversary = {
       var b;
       b <$ {0,1};
       m <@ A.find(pk,c);
-      return if (m = m0) 
+      return if (m = Some m0) 
              then false 
-             else if (m = m1) 
+             else if (m = Some m1) 
                   then true 
                   else b;
    }
@@ -285,7 +289,7 @@ local module Aux = {
    c <@ S.enc(pk, Bow.m0);                                                
    b <$ {0,1};                                                        
    Bow.m <@ A.find(Bow.pk, c);                                           
-   return if Bow.m = Bow.m0 then false else if Bow.m = Bow.m1 then true else b;
+   return if Bow.m = Some Bow.m0 then false else if Bow.m = Some Bow.m1 then true else b;
   }
 
   proc main1() : bool = {
@@ -297,7 +301,7 @@ local module Aux = {
    c <@ S.enc(pk, Bow.m1);                                                
    b <$ {0,1};                                                        
    Bow.m <@ A.find(Bow.pk, c);                                           
-   return if Bow.m = Bow.m0 then false else if Bow.m = Bow.m1 then true else b;
+   return if Bow.m = Some Bow.m0 then false else if Bow.m = Some Bow.m1 then true else b;
   }
 
 }.
@@ -322,72 +326,81 @@ have : Pr[ OW_CPA(S,A).main_perfect() @ &m : res ] <=
 rewrite RField.mulrDr -(pr_CPA_LR S (Bow(A)) &m kg_ll enc_ll); 1,2: by islossless.
 have -> : 
   Pr[CPA_L(S, Bow(A)).main() @ &m : res] = 
-  Pr[CPA_L(S, Bow(A)).main() @ &m : res /\ (Bow.m <> Bow.m0 /\ Bow.m <> Bow.m1)] + 
-  Pr[CPA_L(S, Bow(A)).main() @ &m : res /\ !(Bow.m <> Bow.m0 /\ Bow.m <> Bow.m1)]
-by rewrite Pr[mu_split (Bow.m <> Bow.m0 /\ Bow.m <> Bow.m1)] => /#.
+  Pr[CPA_L(S, Bow(A)).main() @ &m : res /\ (Bow.m = None \/ (Bow.m <> Some Bow.m0 /\ Bow.m <> Some Bow.m1))] + 
+  Pr[CPA_L(S, Bow(A)).main() @ &m : res /\ !(Bow.m = None \/ (Bow.m <> Some Bow.m0 /\ Bow.m <> Some Bow.m1))]
+by rewrite Pr[mu_split (Bow.m = None \/ (Bow.m <> Some Bow.m0 /\ Bow.m <> Some Bow.m1))] => /#.
 
 have -> : 
   Pr[CPA_R(S, Bow(A)).main() @ &m : res] = 
-  Pr[CPA_R(S, Bow(A)).main() @ &m : res /\ (Bow.m <> Bow.m0 /\ Bow.m <> Bow.m1)] + 
-  Pr[CPA_R(S, Bow(A)).main() @ &m : res /\ !(Bow.m <> Bow.m0 /\ Bow.m <> Bow.m1)]
-by rewrite Pr[mu_split (Bow.m <> Bow.m0 /\ Bow.m <> Bow.m1)] => /#.
+  Pr[CPA_R(S, Bow(A)).main() @ &m : res /\ (Bow.m = None \/ (Bow.m <> Some Bow.m0 /\ Bow.m <> Some Bow.m1))] + 
+  Pr[CPA_R(S, Bow(A)).main() @ &m : res /\ !(Bow.m = None \/ (Bow.m <> Some Bow.m0 /\ Bow.m <> Some Bow.m1))]
+by rewrite Pr[mu_split (Bow.m = None \/ (Bow.m <> Some Bow.m0 /\ Bow.m <> Some Bow.m1))] => /#.
 
 have ->  /=: 
-  Pr[CPA_L(S, Bow(A)).main() @ &m : res /\ (Bow.m <> Bow.m0 /\ Bow.m <> Bow.m1)] =
-  Pr[CPA_R(S, Bow(A)).main() @ &m : res /\ (Bow.m <> Bow.m0 /\ Bow.m <> Bow.m1)].
-+ byequiv (: _ ==> (res /\ (Bow.m <> Bow.m0 /\ Bow.m <> Bow.m1)){1} <=>
-                   (res /\ (Bow.m <> Bow.m0 /\ Bow.m <> Bow.m1)){2}) => //.
+  Pr[CPA_L(S, Bow(A)).main() @ &m : res /\ (Bow.m = None \/ (Bow.m <> Some Bow.m0 /\ Bow.m <> Some Bow.m1))] =
+  Pr[CPA_R(S, Bow(A)).main() @ &m : res /\ (Bow.m = None \/ (Bow.m <> Some Bow.m0 /\ Bow.m <> Some Bow.m1))].
++ byequiv (: _ ==> (res /\ (Bow.m = None \/ (Bow.m <> Some Bow.m0 /\ Bow.m <> Some Bow.m1))){1} <=>
+                   (res /\ (Bow.m = None \/ (Bow.m <> Some Bow.m0 /\ Bow.m <> Some Bow.m1))){2}) => //.
   proc. 
   seq 2 2 : (={glob A, glob S, pk,sk, Bow.pk} /\ 
              Bow.m0{1} = Bow.m1{2} /\ Bow.m1{1} = Bow.m0{2} /\ Bow.pk{1} = pk{1} /\
              Bow.m0{1} = m0{1} /\ Bow.m1{1} = m1{1} /\
              Bow.m0{2} = m0{2} /\ Bow.m1{2} = m1{2});
      1: by inline *;swap {1} 4 1;auto;call(_: true); auto.
-  by inline *;wp;call(_: true);rnd;wp;call(_:true);auto => />.
+  by inline *;wp;call(_: true);rnd;wp;call(_:true);auto => /> /#.
 
 have : 
-   Pr[CPA_L(S, Bow(A)).main() @ &m : res /\ ! (Bow.m <> Bow.m0 /\ Bow.m <> Bow.m1)] <= eps_msg.
-+ have -> : Pr[CPA_L(S, Bow(A)).main() @ &m : res /\ ! (Bow.m <> Bow.m0 /\ Bow.m <> Bow.m1)] = 
-            Pr[Aux.main0() @ &m : res /\ ! (Bow.m <> Bow.m0 /\ Bow.m <> Bow.m1)]
+   Pr[CPA_L(S, Bow(A)).main() @ &m : res /\ ! (Bow.m = None \/ (Bow.m <> Some Bow.m0 /\ Bow.m <> Some Bow.m1))] <= eps_msg.
++ have -> : Pr[CPA_L(S, Bow(A)).main() @ &m : res /\ ! (Bow.m = None \/ (Bow.m <> Some Bow.m0 /\ Bow.m <> Some Bow.m1))] = 
+            Pr[Aux.main0() @ &m : res /\ ! (Bow.m = None \/ (Bow.m <> Some Bow.m0 /\ Bow.m <> Some Bow.m1))]
    by byequiv => //;proc;inline *;wp;conseq />; sim. 
   byphoare => //. 
   proc;inline *; swap 4 3.
-  conseq (: _ ==> Bow.m1 = Bow.m); 1: by smt().
+  conseq (: _ ==> Some Bow.m1 = Bow.m); 1: by smt().
   seq 6 : true  (1%r)  (eps_msg) (0%r) (0%r).
   + by trivial.
   + by trivial. 
-  + by rnd; skip => /> *;rewrite eps_msgE /#.
-  + by hoare; trivial.
+  + rnd; skip => /> &hr.  
+    case(Bow.m{hr} = None); 1: by move => -> /=; rewrite mu0;smt(MFinT.card_gt0).
+    move => nnone.
+    have -> : (fun (x : plaintext) => Some x = Bow.m{hr})  = pred1 (oget Bow.m{hr}) by apply fun_ext => x;smt().
+    by smt(eps_msgE).
+     + by hoare; trivial.
   by trivial.
   
 have : 
   `| Pr[OW_CPA(S, A).main_perfect() @ &m : res] - 
-      Pr[CPA_R(S, Bow(A)).main() @ &m : res /\ ! (Bow.m <> Bow.m0 /\ Bow.m <> Bow.m1)]| <= 
-         eps_msg.
-+ have -> : Pr[OW_CPA(S, A).main_perfect() @ &m : res] = 
-            Pr[Aux.main1()           @ &m : Bow.m = Bow.m1].
+      Pr[CPA_R(S, Bow(A)).main() @ &m : res /\ ! (Bow.m = None \/ (Bow.m <> Some Bow.m0 /\ Bow.m <> Some Bow.m1))]| <= 
+         eps_msg; last by smt().
+
+have -> : Pr[OW_CPA(S, A).main_perfect() @ &m : res] = 
+            Pr[Aux.main1()           @ &m : Bow.m = Some Bow.m1]
      by byequiv => //;proc;inline*;wp;call(_: true);rnd{2};
         call(:true);rnd;rnd{2};wp;call(_: true);auto => />.
 
-  have -> : Pr[CPA_R(S, Bow(A)).main() @ &m : res /\ ! (Bow.m <> Bow.m0 /\ Bow.m <> Bow.m1)] = 
-            Pr[Aux.main1()           @ &m : res /\ ! (Bow.m <> Bow.m0 /\ Bow.m <> Bow.m1)];
-     1: by byequiv => //;proc;inline*;wp;conseq />;sim.
-  have <- : Pr[Aux.main1() @ &m : !res /\ ! (Bow.m <> Bow.m0 /\ Bow.m <> Bow.m1)] = 
+have -> : Pr[CPA_R(S, Bow(A)).main() @ &m : res /\ ! (Bow.m = None \/ (Bow.m <> Some Bow.m0 /\ Bow.m <> Some Bow.m1))] = 
+            Pr[Aux.main1()           @ &m : res /\ ! (Bow.m = None \/ (Bow.m <> Some Bow.m0 /\ Bow.m <> Some Bow.m1))]
+      by byequiv => //;proc;inline*;wp;conseq />;sim.
+
+  have  : Pr[Aux.main1() @ &m : !res /\  !(Bow.m <> Some Bow.m0 /\ Bow.m <> Some Bow.m1)] <= 
             eps_msg.
   + byphoare => //. 
     proc;inline *;swap 3 4.
-    conseq (: _ ==> Bow.m0 = Bow.m); 1: by smt().
+    conseq (: _ ==> Bow.m0 = oget Bow.m); 1: by smt().
     seq 6 : true  (1%r)  (eps_msg) (0%r) (0%r).
     + by trivial.
     + by islossless. 
-    + by rnd; skip => /> *;rewrite eps_msgE /#.
+    + rnd; skip => />*; rewrite eps_msgE /#.
     + by hoare; trivial. 
-    by trivial.
-  byequiv : (!res /\ ! (Bow.m <> Bow.m0 /\ Bow.m <> Bow.m1)) => //. 
+    by trivial. 
+
+  have : `|Pr[Aux.main1() @ &m : Bow.m = Some Bow.m1] -
+  Pr[Aux.main1() @ &m : res /\ ! (Bow.m = None \/ Bow.m <> Some Bow.m0 /\ Bow.m <> Some Bow.m1)]|  <=
+      Pr[Aux.main1() @ &m : !res /\ ! (Bow.m <> Some Bow.m0 /\ Bow.m <> Some Bow.m1)]; last by smt().
+  byequiv : (!res /\ ! (Bow.m = None \/ (Bow.m <> Some Bow.m0 /\ Bow.m <> Some Bow.m1))) => //. 
   + proc;inline *.
-    by call(:true);rnd;call(:true);rnd;rnd;wp;call(:true);auto => />.
+    by call(:true);rnd;call(:true);rnd;rnd;wp;call(:true);auto => /> /#.
     
-by smt().
 qed.
 
 end section.
@@ -596,7 +609,7 @@ module type VA_ORC = {
 }.
 
 module type PCVA_ADV (H : POracle, O: VA_ORC) = {
-  proc find(pk : pkey, c:ciphertext) : plaintext 
+  proc find(pk : pkey, c:ciphertext) : plaintext option
 }.
 
 op [lossless] dplaintext : plaintext distr.
@@ -625,7 +638,8 @@ module OW_PCVA (H : Oracle, S:Scheme, A: PCVA_ADV) = {
 
   proc main() : bool = {
     var pk : pkey;
-    var m, m' : plaintext;
+    var m  : plaintext;
+    var m' : plaintext option;
     var b;
 
     H.init();
@@ -633,8 +647,8 @@ module OW_PCVA (H : Oracle, S:Scheme, A: PCVA_ADV) = {
     m        <$ dplaintext;
     cc       <@ S(H).enc(pk, m);
     m'       <@ A.find(pk,cc);
-    b        <@ O.pco(m',cc);
-    return b;
+    b        <@ O.pco(oget m',cc);
+    return if m' = None then false else b;
   }
 }.
 
